proof/uniform_binary_choice/BinUniSample_proof.ec
@@ -1,0 +1,260 @@
+require import AllCore IntDiv CoreMap List Distr DList.
+from Jasmin require import JModel.
+
+require import Array32.
+require BinUniSample_spec.
+require import Array1 WArray1.
+require import Finite FinLists.
+
+require import BigNum_proofs.
+require import W64_SchnorrExtract.
+
+
+clone import BinUniSample_spec as BUS with type t <- W64.t Array32.t
+proof*.
+
+section.
+
+local op h = (fun (a : WArray1.t) => Array1.init (fun i => WArray1.get8 a i)).
+
+local lemma init_ext:
+  forall (f1 f2 : int -> W8.t),
+       (Array1.init f1) = (Array1.init f2) =>
+    (forall (x : int), 0 <= x && x < 1 => f1 x = f2 x).
+smt(@Array1).
+qed.
+
+
+local lemma h_inj : injective h.
+rewrite /injective.
+rewrite /h. 
+move => x y  q.
+have :  get8 x 0 =  get8 y 0.
+apply  (init_ext _ _ q 0 _). smt().
+rewrite /get8. smt(@WArray1).
+qed.
+
+
+local lemma h_surj : surjective h.    
+rewrite /surjective.
+progress. 
+exists (WArray1.init (fun i => x.[i])).
+rewrite /h.
+apply Array1.ext_eq.
+progress. have ->: x0 = 0. smt().
+smt(@Array1 @WArray1).
+qed.
+
+
+
+local lemma darray_ll:
+ is_lossless darray.
+proof. rewrite /darray. apply dmap_ll; apply dlist_ll. smt(@W8). qed.
+
+
+local lemma supp_darray a:
+ a \in darray <=> all (support W8.dword) (WArray1.to_list a).
+proof.
+rewrite /darray128 supp_dmap; split.
+ move=> [x]; rewrite supp_dlist // => /> *.
+ by rewrite WArray1.of_listK // /#.
+move=> H; exists (to_list a); rewrite supp_dlist // H Array256.size_to_list /=.
+qed.
+
+
+local lemma darray_uni:
+   is_uniform (darray).
+proof.
+rewrite /darray1=> ?; apply dmap_uni_in_inj.
+ move=> x y; rewrite !supp_dlist //; move => [? _] [? _] H.
+  smt(@WArray1).
+ apply dlist_uni. smt(@W8).
+qed.
+
+
+local lemma darray_fu:
+   is_full darray.
+proof.
+rewrite /darray => H; apply dmap_fu_in.
+move=> x; exists (to_list x); rewrite to_listK supp_dlist //=.
+rewrite allP.
+progress. smt(@W8).
+qed.
+
+local op byte_distr = dmap WArray1.darray h.
+
+local lemma byte_distr_uni : is_uniform byte_distr .
+rewrite /jsmD.
+apply dmap_uni_in_inj.
+progress. smt (h_inj).
+apply darray_uni.
+qed.
+
+
+local lemma byte_distr_ll: is_lossless byte_distr.
+rewrite /jsmD.
+apply dmap_ll.
+apply darray_ll.
+qed.
+
+local lemma byte_distr_fu : is_full byte_distr .
+rewrite /jsmD.
+apply dmap_fu.
+smt (h_surj).
+apply darray_fu.
+qed.
+
+
+
+
+local module SampleModule = {
+  proc byte_distr() = {
+    var r;
+    r <$ byte_distr;
+    return r;
+  }
+
+  proc bit_distr() = {
+    var b;
+    b <@ byte_distr();
+    b.[0] <- (b.[0] `&` (W8.of_int 1));
+    return b.[0];
+  }
+
+
+}.
+
+
+
+local lemma zzz : size (to_seq (support byte_distr)) =  256.
+have : size all_256words1 = size (to_seq (support byte_distr)).
+apply uniq_size_uniq.
+apply uniq_to_seq.
+smt(@Distr byte_distr_uni).
+progress. apply all_256words1_full.
+have : x \in byte_distr.
+apply byte_distr_fu.
+smt.
+apply all_256words1_uniq.
+progress. rewrite - H.
+rewrite all_256words1_size. smt().
+qed.
+
+local op toi (x : W8.t Array1.t) : int = W8.to_uint x.[0].
+local op fri (x : int) : W8.t Array1.t   = (Array1.init (fun i => (W8.of_int x))).
+local lemma lemma2 : 
+  equiv [SampleModule.byte_distr ~ BinSampleSpec.sampleInt : true ==> toi res{1} = res{2} ].
+proc.
+rnd  toi fri.
+skip. progress.
+rewrite /toi /fri. 
+smt.
+rewrite duniform1E_uniq. smt(@List).
+have ->: xR \in range 0 (255 + 1). smt(@List @Distr).
+simplify. 
+have ->: size (range 0 256) = 256. smt(@List).
+rewrite mu1_uni. apply byte_distr_uni.
+rewrite byte_distr_fu. simplify.
+rewrite byte_distr_ll. 
+rewrite zzz. auto.
+have : 0 <= toi rL < 256. rewrite /toi. 
+have ->: 256 = W8.modulus. ring.
+apply W8.to_uint_cmp.
+smt(@Distr).
+rewrite /fri /toi.
+apply Array1.ext_eq.
+progress.
+have ->: x = 0. smt().
+simplify. auto.
+qed.
+
+local lemma lemma3 : 
+  equiv [SampleModule.bit_distr ~ BinSampleSpec.run : true ==>  W8.to_uint res{1} = res{2} ].
+proc.
+wp. call lemma2. skip. progress.
+rewrite /toi. 
+have ->: W8.one = (W8.of_int (2 ^ 1 - 1)). simplify. auto.
+rewrite (W8.and_mod 1 result_L.[0] _ ). auto. simplify. smt(@IntDiv).
+qed.
+
+
+
+local module W = {
+  proc step1()  = {
+    var byte_p : W8.t Array1.t;
+    var _byte_p : W8.t Array1.t;
+    var r : W8.t;
+    _byte_p <- byte_p;
+    byte_p <@ Syscall.randombytes_1(_byte_p);
+    r <- byte_p.[0];
+    r <- r `&` W8.one;    
+    return r;
+  }
+ 
+  proc step2(a b : W64.t Array32.t) = {
+    var r, cond;
+    r <@ step1();
+    cond <- r = W8.zero;
+    a <@ M(Syscall).bn_cmov(cond, b, a);
+    return a;
+  }
+}.
+
+local lemma lemma4 : 
+  equiv [W.step1 ~ BinSampleSpec.run : true ==>  W8.to_uint res{1} = res{2} ].
+transitivity SampleModule.bit_distr
+ (true ==> res{1} = res{2})
+ (true ==> W8.to_uint res{1} = res{2}).
+auto. auto.
+proc. wp.
+inline*.
+wp. rnd. wp.
+skip. progress.
+conseq lemma3.
+qed.
+
+
+
+
+local lemma lemma5 : 
+  equiv [W.step2 ~ BinSampleSpec.main : ={arg} ==>   res{1} = res{2} ].
+proc. 
+wp.
+ecall {1} (bn_cmov_correct cond{1} b{1} a{1}).
+wp. 
+call lemma4.
+skip. progress.
+smt(@W8).
+qed.
+
+
+
+local lemma lemma6 : 
+  equiv [W.step2 ~ BinSampleSpec.spec : ={arg} ==>   res{1} = res{2} ].
+symmetry.
+transitivity BinSampleSpec.main
+  (={arg} ==> ={res})
+  (={arg} ==> ={res}).
+progress. smt(). auto.
+symmetry.
+proc*. ecall (sat_spec a{1} b{1}). skip. auto.
+symmetry.
+conseq lemma5.
+auto. auto.
+qed.
+
+
+
+lemma uniform_binary_choice_eq : 
+  equiv [M(Syscall).uniform_binary_choice ~ BinSampleSpec.spec : ={arg} ==> res{1} = res{2} ].
+transitivity W.step2
+  (={arg} ==> ={res})
+  (={arg} ==> ={res}).
+smt(). smt().
+proc. wp.
+call (_:true). sim. wp.
+inline*. wp.  rnd. wp.  skip. progress.
+conseq lemma6.
+qed.
+
+end section.
